Proofs of some basic properties.

StateSpaceTheorems.v
@@ -17,31 +17,223 @@ Require Import Coq.Sets.Ensembles.
 Variable Scalar : Type.
 Variable State : Type.
 
-Definition equal_inner_prod_forall
- {statespace : StateSpace Scalar State}
- (S1 S2 : State) (S0 : State) := <| S0 | S1 |> = <| S0 | S2 |>.
-
-Definition state_join_bot
+(* Inductive equality for meets and joins.  This, combined with a
+ * basis equality lemma, will become the primary proof goal for showing
+ * equality. *)
+Definition state_meet_join_ind_eq
   {statespace : StateSpace Scalar State}
-  (s : State) := join null s = s.
+  (S1 S2 : State) : Prop :=
+  (forall (S3 S4 : State),
+    <| S3 | S1 |> = <| S3 | S2 |> -> <| S4 | S1 |> = <| S4 | S2 |> ->
+      <| join S3 S4 | S1 |> = <| join S3 S4 | S2 |>) /\
+  (forall (S3 S4 : State),
+    <| S3 | S1 |> = <| S3 | S2 |> -> <| S4 | S1 |> = <| S4 | S2 |> ->
+      <| meet S3 S4 | S1 |> = <| meet S3 S4 | S2 |>).
 
-Lemma state_join_bot_inductive
-  {statespace : StateSpace Scalar State} :
-  state_pred_inductive state_join_bot.
+(* Helper for proving that extensional equality on inner products is
+ * inductive *)
+Definition state_inner_prod_eq
+  {statespace : StateSpace Scalar State}
+  (S1 S2 : State) (S : State) :=
+   <| S | S1 |> = <| S | S2 |>.
+
+(* If we have meet-join inductive equality, we can show that full
+ * extensional equality is inductive *)
+Lemma state_inner_prod_eq_ind
+  {statespace : StateSpace Scalar State}
+  (S1 S2 : State) :
+  state_meet_join_ind_eq S1 S2 ->
+  state_pred_inductive (state_inner_prod_eq S1 S2).
 Proof.
+  unfold state_meet_join_ind_eq.
+  intros (join_ind & meet_ind).
   unfold state_pred_inductive.
-  unfold state_join_bot.
+  unfold state_inner_prod_eq.
+  split.
+  assumption.
+  split.
+  assumption.
   split.
   intros.
-  apply inner_prod_ext_eq.
+  rewrite 2! inner_prod_left_homogeneous.
+  apply mul_extensional.
+  reflexivity.
+  assumption.
+  exact innerprod_ss.
+  exact innerprod_ss.
+  split.
   intros.
-  rewrite inner_prod_left_join.
+  (* Appeal to actual definitions of complex numbers, which I haven't
+   * developed here yet.  Eventually develop them, come back, and get rid
+   * of this. *)
+  admit.
+  rewrite 2! inner_prod_left_strict.
+  reflexivity.
+  exact innerprod_ss.
+  exact innerprod_ss.
+Qed.
+
+(* Basis equality: Are these two states equal in an inner product with
+ * any basis element? *)
+Definition state_basis_eq
+  {statespace : StateSpace Scalar State}
+  (B : Ensemble State) (S1 S2 : State) : Prop :=
+  forall (S : State), In State B S -> <| S | S1 |> = <| S | S2 |>.
+
+(* If we have a basis for the entire state space, then meet-join
+ * equality and basis equality proves general equality. *)
+Lemma state_meet_join_eq_induction_with_basis
+  {statespace : StateSpace Scalar State}
+  (B : Ensemble State) (S1 S2 : State) :
+  (forall (S : State), state_basis B S) ->
+  state_meet_join_ind_eq S1 S2 ->
+  state_pred_forall_basis B (state_inner_prod_eq S1 S2) ->
+  S1 = S2.
+Proof.
+  intros.
   apply inner_prod_ext_eq.
+  intro.
+  apply (state_inner_prod_eq_ind S1 S2) in H0.
+  apply (state_basis_induction B (state_inner_prod_eq S1 S2)).
+  assumption.
+  assumption.
+  apply H.
+Qed.
+
+(* join S1 S2 = join S2 S1 *)
+Lemma state_join_comm_meet_join_eq
+  {statespace : StateSpace Scalar State} :
+  forall (S1 S2 : State), state_meet_join_ind_eq (join S1 S2) (join S2 S1).
+Proof.
+  intro.
+  unfold state_meet_join_ind_eq.
+  split.
+  intros.
+  rewrite 2! inner_prod_join_right.
+  rewrite add_comm.
+  reflexivity.
+  intros.
+  rewrite 2! inner_prod_meet_join.
+  apply mul_extensional.
+  rewrite add_comm.
+  reflexivity.
+  rewrite add_comm.
+  reflexivity.
+  exact innerprod_ss.
+  exact innerprod_ss.
+Qed.
+
+Lemma state_meet_comm_meet_join_eq
+  {statespace : StateSpace Scalar State} :
+  forall (S1 S2 : State), state_meet_join_ind_eq (meet S1 S2) (meet S2 S1).
+Proof.
+  intro.
+  unfold state_meet_join_ind_eq.
+  split.
+  intros.
+  rewrite 2! inner_prod_right_meet.
+  apply mul_comm.
+  intros.
+  rewrite 2! inner_prod_right_meet.
+  apply mul_comm.
+Qed.
+
+(*
+Lemma state_join_assoc_meet_join_eq
+  {statespace : StateSpace Scalar State} :
+  forall (S1 S2 S3 : State),
+    state_meet_join_ind_eq (join (join S1 S2) S3) (join S1 (join S2 S3)).
+Proof.
+  intro.
+  unfold state_meet_join_ind_eq.
+  split.
+  intros.
+  rewrite 4! inner_prod_join_right.
+  rewrite add_assoc.
+  reflexivity.
+  intros.
+  rewrite 2! inner_prod_meet_join.
+
+Lemma state_meet_assoc_meet_join_eq
+  {statespace : StateSpace Scalar State} :
+  forall (S1 S2 S3 : State),
+    state_meet_join_ind_eq (meet (meet S1 S2) S3) (meet S1 (meet S2 S3)).
+Proof.
+  intro.
+  unfold state_meet_join_ind_eq.
+  split.
+  intros.
+*)
+
+(* join null S = S *)
+Lemma state_join_bot_meet_join_eq
+  {statespace : StateSpace Scalar State} :
+  forall (S : State), state_meet_join_ind_eq (join null S) S.
+Proof.
+  intro.
+  unfold state_meet_join_ind_eq.
+  split.
   intros.
   rewrite inner_prod_join_right.
   rewrite inner_prod_right_strict.
-  rewrite add_zero_left.
+  rewrite add_comm.
+  rewrite add_zero_right.
   reflexivity.
+  intros.
+  rewrite inner_prod_meet_join.
+  rewrite 2! inner_prod_right_strict.
+  rewrite add_comm.
+  rewrite add_zero_right.
+  rewrite add_comm.
+  rewrite add_zero_right.
+  rewrite inner_prod_left_meet.
+  reflexivity.
+  exact innerprod_ss.
+  exact innerprod_ss.
 Qed.
 
+(* meet null S = null *)
+Lemma state_meet_bot_meet_join_eq
+  {statespace : StateSpace Scalar State} :
+  forall (S : State), state_meet_join_ind_eq (meet null S) null.
+Proof.
+  intro.
+  unfold state_meet_join_ind_eq.
+  split.
+  intros.
+  rewrite inner_prod_join_meet.
+  rewrite 3! inner_prod_right_strict.
+  rewrite add_zero_right.
+  rewrite mul_comm.
+  rewrite mul_zero_right.
+  reflexivity.
+  intros.
+  rewrite inner_prod_right_meet.
+  rewrite inner_prod_right_strict.
+  rewrite mul_comm.
+  rewrite mul_zero_right.
+  reflexivity.
+Qed.
+(*
+Lemma state_join_scalar_meet_join_eq
+  {statespace : StateSpace Scalar State} :
+  forall (S : State) (a b : Scalar),
+    state_meet_join_ind_eq (join (scalar_prod a S) (scalar_prod b S))
+                           (scalar_prod (a + b) S).
+Proof.
+  intro.
+  unfold state_meet_join_ind_eq.
+  split.
+  intros.
+  rewrite inner_prod_join_right.
+  rewrite 3! inner_prod_right_homogeneous.
+  rewrite mul_comm.
+  replace (b * <| join S3 S4 | S |>) with (<| join S3 S4 | S |> * b).
+  rewrite <- add_mul_dist.
+  apply mul_comm.
+  apply mul_comm.
+  intros.
+  rewrite inner_prod_meet_join.
+  rewrite 5! inner_prod_right_homogeneous.
+*)
 End StateSpaceTheorems.
